iris/UexecRound.v
@@ -78,26 +78,28 @@ Definition uround_bump_ok (tf tf' : list (mword 64)) (r : mword 64) : Prop :=
 (* ===================================================================== *)
 Definition uround_ok (sc : mword 64)
     (tf : list (mword 64)) (M : gmap Z (bv 8)) (pi : gmap (mword 27) uperm)
-    (tf' : list (mword 64)) (M' : gmap Z (bv 8)) (pi' : gmap (mword 27) uperm) : Prop :=
+    (szv : Z)
+    (tf' : list (mword 64)) (M' : gmap Z (bv 8)) (pi' : gmap (mword 27) uperm)
+    (szv' : Z) : Prop :=
   if decide (sc = uecall_scause) then
     usys_num tf = USYS_exec
     \/ (usys_num tf <> USYS_exit
         /\ exists r : mword 64,
              uround_bump_ok tf tf' r
-             /\ usys_mem_ok (usys_num tf) tf r M pi M' pi')
-  else uround_id_ok tf tf' /\ M' = M /\ pi' = pi.
+             /\ usys_mem_ok (usys_num tf) tf r M pi szv M' pi' szv')
+  else uround_id_ok tf tf' /\ M' = M /\ pi' = pi /\ szv' = szv.
 
 (* ===================================================================== *)
 (* SS3 The readers -- unpack the [decide].                                 *)
 (* ===================================================================== *)
 Lemma uround_ok_ecall (tf : list (mword 64)) (M M' : gmap Z (bv 8))
-    (pi pi' : gmap (mword 27) uperm) (tf' : list (mword 64)) :
-  uround_ok uecall_scause tf M pi tf' M' pi' ->
+    (pi pi' : gmap (mword 27) uperm) (szv szv' : Z) (tf' : list (mword 64)) :
+  uround_ok uecall_scause tf M pi szv tf' M' pi' szv' ->
   usys_num tf = USYS_exec
   \/ (usys_num tf <> USYS_exit
       /\ exists r : mword 64,
            uround_bump_ok tf tf' r
-           /\ usys_mem_ok (usys_num tf) tf r M pi M' pi').
+           /\ usys_mem_ok (usys_num tf) tf r M pi szv M' pi' szv').
 Proof.
   unfold uround_ok.
   destruct (decide (uecall_scause = uecall_scause)) as [_ | Hne];
@@ -105,11 +107,11 @@ Proof.
 Qed.
 
 Lemma uround_ok_transparent (sc : mword 64) (tf : list (mword 64))
-    (M M' : gmap Z (bv 8)) (pi pi' : gmap (mword 27) uperm)
+    (M M' : gmap Z (bv 8)) (pi pi' : gmap (mword 27) uperm) (szv szv' : Z)
     (tf' : list (mword 64)) :
   sc <> uecall_scause ->
-  uround_ok sc tf M pi tf' M' pi' ->
-  uround_id_ok tf tf' /\ M' = M /\ pi' = pi.
+  uround_ok sc tf M pi szv tf' M' pi' szv' ->
+  uround_id_ok tf tf' /\ M' = M /\ pi' = pi /\ szv' = szv.
 Proof.
   intros Hne. unfold uround_ok.
   destruct (decide (sc = uecall_scause)) as [Heq | _];
@@ -124,10 +126,11 @@ Qed.
 (* [tf'].                                                                  *)
 (* ===================================================================== *)
 Lemma uround_ok_ueq_l (sc : mword 64) (tf tfa : list (mword 64))
-    (M M' : gmap Z (bv 8)) (pi pi' : gmap (mword 27) uperm)
+    (M M' : gmap Z (bv 8)) (pi pi' : gmap (mword 27) uperm) (szv szv' : Z)
     (tf' : list (mword 64)) :
   tf_ueq tf tfa ->
-  uround_ok sc tf M pi tf' M' pi' -> uround_ok sc tfa M pi tf' M' pi'.
+  uround_ok sc tf M pi szv tf' M' pi' szv'
+  -> uround_ok sc tfa M pi szv tf' M' pi' szv'.
 Proof.
   intros Hu H.
   pose proof (tf_ueq_num tf tfa Hu) as Hn.
@@ -141,7 +144,8 @@ Proof.
     + right. split; [ rewrite <- Hn; exact Hnx | ]. exists r. split; [ split | ].
       * rewrite <- Hg. exact Hb1.
       * unfold tf_w in Hb2 |- *. rewrite <- He. exact Hb2.
-      * rewrite <- Hn. exact (usys_mem_ok_ueq (usys_num tf) tf tfa r M M' pi pi' Hu Hm).
+      * rewrite <- Hn.
+        exact (usys_mem_ok_ueq (usys_num tf) tf tfa r M M' pi pi' szv szv' Hu Hm).
   - destruct H as [[Hi1 Hi2] Hrest].
     split; [ split | exact Hrest ].
     + rewrite <- Hg. exact Hi1.
@@ -149,10 +153,11 @@ Proof.
 Qed.
 
 Lemma uround_ok_ueq_r (sc : mword 64) (tf : list (mword 64))
-    (M M' : gmap Z (bv 8)) (pi pi' : gmap (mword 27) uperm)
+    (M M' : gmap Z (bv 8)) (pi pi' : gmap (mword 27) uperm) (szv szv' : Z)
     (tf' tfa' : list (mword 64)) :
   tf_ueq tf' tfa' ->
-  uround_ok sc tf M pi tf' M' pi' -> uround_ok sc tf M pi tfa' M' pi'.
+  uround_ok sc tf M pi szv tf' M' pi' szv'
+  -> uround_ok sc tf M pi szv tfa' M' pi' szv'.
 Proof.
   intros Hu H.
   pose proof (tf_ueq_resume_gpr0 tf' tfa' Hu) as Hg.
